examples/data_structures/binary_search_tree.fst
@@ -1,41 +1,79 @@
-module BST
+(*
+   Copyright 2008-2014 Nikhil Swamy and Microsoft Research
 
-let max i j = if i < j then j else i
+   Licensed under the Apache License, Version 2.0 (the "License");
+   you may not use this file except in compliance with the License.
+   You may obtain a copy of the License at
+
+       http://www.apache.org/licenses/LICENSE-2.0
+
+   Unless required by applicable law or agreed to in writing, software
+   distributed under the License is distributed on an "AS IS" BASIS,
+   WITHOUT WARRANTIES OR CONDITIONS OF ANY KIND, either express or implied.
+   See the License for the specific language governing permissions and
+   limitations under the License.
+*)
+
+(* 
+   Exercising:
+    -- indexed types
+    -- implicit value parameters
+    -- dependent tuples
+    -- and refinements, of course
+ *)
+
+module BST
 
 (* The type of a binary tree indexed by its max element *)
 type tree: int -> Type = 
-  | Leaf : n:int -> tree n
-  | Node : #l:int -> left:option (tree l)
-        ->  n:int
-        -> #r:int -> right:option (tree r){l <= n 
-                                            /\ n <= r 
-                                            /\ (is_None right <==> n=r)
-                                            /\ (is_None left <==> n=l)}
+  | Node : #l   :int 
+        -> left :option (tree l)
+        -> n    :int
+        -> #r   :int 
+        -> right:option (tree r){l <= n 
+                                 /\ n <= r 
+                                 /\ (is_None right <==> n=r)
+                                 /\ (is_None left <==> n=l)}
         -> tree r
-    
+
+let leaf i = Node #i None i #i None (* Need to supply #i for the empty sub-trees, since it can't be inferred by unification *)
+let max i j = if i < j then j else i
 
 val insert: #k:int -> t:tree k -> i:int -> Tot (tree (max k i)) (decreases t)
-let rec insert k t i = match t with 
-  | Leaf n -> 
-    if i = n
-    then t
-    else if i < n 
-    then Node (Some (Leaf i)) n #n None 
-    else Node #n None n (Some (Leaf i))
+let rec insert k (Node left n right) i =
+  if i = n
+  then Node left n right
+  else if i < n
+  then match left with
+       | None ->
+          Node (Some (leaf i)) n right
+       | Some left ->
+          Node (Some (insert left i)) n right
+  else match right with
+       | None ->
+          Node left n (Some (leaf i))
+       | Some right ->
+          Node left n (Some (insert right i))
+               
+val contains: #k:int -> t:tree k -> key:int -> Tot bool (decreases t)
+let rec contains k t key =
+  if key > k
+  then false
+  else let Node left i right = t in
+       i=k
+       || (key < i && is_Some left && contains (Some.v left) key)
+       || (is_Some right && contains (Some.v right) key)
 
-  | Node #l left n #r right -> 
-    if i = n 
-    then t
-    else if i < n
-    then match left with 
-      | None -> 
-        Node (Some (Leaf i)) n right
-      | Some left -> 
-        let left' = insert left i in 
-        Node (Some left') n right
-    else match right with 
-      | None -> 
-        Node left n (Some (Leaf i))
-      | Some right -> 
-        let right' = insert right i in
-        Node left n (Some right')
+val in_order: #k:int -> t:tree k -> Tot (list int) (decreases t)
+let rec in_order k (Node left i right) =
+  let l = match left with
+    | None -> []
+    | Some left -> in_order left in
+  let r = match right with
+    | None -> []
+    | Some right -> in_order right in
+  l@[i]@r
+
+type t = (|l:int * tree l|)                        (* The lens-bracketed tuple is sugar for DTuple2 int (fun (l:int) -> tree l) *)
+val ins : lt:t -> n:int -> Tot t
+let ins (| m, tt |) n = (| max m n, insert tt n |) (* open the dependent pair by matching it; repackage it, using the expected type t from the annotation *)
